test

basis/pure/.hol/make-deps/basisComputeLib.sig.d
@@ -1,0 +1,1 @@
+basisComputeLib.ui: /Users/matthewrichards/projects/HOL/sigobj/computeLib.uo 
