basis/pure/.hol/make-deps/basisComputeLib.sml.d
@@ -1,0 +1,1 @@
+basisComputeLib.uo: basisComputeLib.ui /Users/matthewrichards/projects/HOL/sigobj/Parse.uo /Users/matthewrichards/projects/HOL/sigobj/computeLib.uo mlintTheory.uo mloptionTheory.uo mlstringTheory.uo 
