basis/pure/.hol/make-deps/mllistScript.sml.d
@@ -1,0 +1,1 @@
+mllistScript.uo: /Users/matthewrichards/projects/HOL/sigobj/DB_dtype.uo /Users/matthewrichards/projects/HOL/sigobj/Q.uo /Users/matthewrichards/projects/HOL/sigobj/TotalDefn.uo /Users/matthewrichards/projects/HOL/sigobj/boolLib.uo /Users/matthewrichards/projects/cakeml/misc/preamble.uo /Users/matthewrichards/projects/HOL/src/sort/ternaryComparisonsTheory.uo 
