basis/pure/.hol/make-deps/mlsetScript.sml.d
@@ -1,0 +1,1 @@
+mlsetScript.uo: /Users/matthewrichards/projects/HOL/sigobj/DB_dtype.uo /Users/matthewrichards/projects/HOL/sigobj/TotalDefn.uo /Users/matthewrichards/projects/HOL/examples/data-structures/balanced_bst/balanced_mapTheory.uo /Users/matthewrichards/projects/HOL/sigobj/bossLib.uo /Users/matthewrichards/projects/cakeml/misc/preamble.uo 
