basis/pure/.hol/make-deps/mlstringSyntax.sig.d
@@ -1,0 +1,1 @@
+mlstringSyntax.ui: /Users/matthewrichards/projects/HOL/sigobj/Abbrev.uo 
