candle/standard/syntax/.hol/make-deps/holSyntaxSyntax.sml.d
@@ -1,0 +1,1 @@
+holSyntaxSyntax.uo: /Users/matthewrichards/projects/HOL/sigobj/HolKernel.uo holSyntaxTheory.uo 
