semantics/.hol/make-deps/semanticsScript.sml.d
@@ -1,0 +1,1 @@
+semanticsScript.uo: /Users/matthewrichards/projects/HOL/sigobj/DB_dtype.uo /Users/matthewrichards/projects/HOL/sigobj/TotalDefn.uo /Users/matthewrichards/projects/HOL/sigobj/bossLib.uo cmlPtreeConversionTheory.uo lexer_funTheory.uo /Users/matthewrichards/projects/cakeml/misc/preamble.uo primTypesTheory.uo 
