semantics/.hol/make-deps/tokenUtilsScript.sml.d
@@ -1,0 +1,1 @@
+tokenUtilsScript.uo: /Users/matthewrichards/projects/HOL/sigobj/DB_dtype.uo /Users/matthewrichards/projects/HOL/sigobj/Q.uo /Users/matthewrichards/projects/HOL/sigobj/TotalDefn.uo /Users/matthewrichards/projects/HOL/examples/formal-languages/context-free/grammarTheory.uo /Users/matthewrichards/projects/cakeml/misc/preamble.uo tokensTheory.uo 
